Added a new lemma about the behavior of a program at a fixpoint. Proved divergence of a sample program.

URM.v
@@ -24,9 +24,13 @@ Fixpoint nth_d (l:list nat) (d n:nat) : nat :=
   | _ :: l', S n' => nth_d l' d n'
 end.
 
-(* Implements an unbounded register file. *)
-Definition set_init_conf (c:list nat) : config :=
-  (0, fun (x:nat) => nth_d c 0 x).
+(* Notation for config literals from a list *)
+Notation "$ X" := 
+    (fun (x:nat) => nth_d X 0 x) 
+    (at level 75, right associativity).
+
+Check (0, $[5,2,3]):config.   
+
 
 
 (* Replace the n'th register. *)
@@ -79,7 +83,7 @@ end.
 
 (* Definition of a terminal state (PC at end of program) *)
 Definition Final (p:program) (c:config) : bool :=
-  beq_nat (fst c) (length p).
+  beq_nat (length p) (fst c).
 
 
 (* Nth instruction (or a default) *)
@@ -113,15 +117,15 @@ end.
 (* With stepping functions and a terminal condtion defined,
  we can define propositions for HALT and DIVERGE, etc. *)
 
-Definition HALTS (P:program) (l:list nat) : Prop :=
-  exists n:nat, true = (Final P (EXEC_STEPS n P (set_init_conf l))).
+Definition HALTS (P:program) (c:config) : Prop :=
+  exists n:nat, true = (Final P (EXEC_STEPS n P c)).
 
-Definition DIVERGES (P:program) (l:list nat) : Prop :=
-  ~ HALTS P l.
+Definition DIVERGES (P:program) (c:config) : Prop :=
+  ~ HALTS P c.
 
 
-Definition STP (P:program) (l:list nat) (t:nat): Prop :=
-  true = Final P (EXEC_STEPS t P (set_init_conf l)).
+Definition STP (P:program) (c:config) (t:nat): Prop :=
+  true = Final P (EXEC_STEPS t P c).
 
 
 
@@ -132,16 +136,47 @@ Definition STP (P:program) (l:list nat) (t:nat): Prop :=
 
 (* This halts in three steps. Easy. *)
 Check ([ZR 0]).
-Example conv0 : STP [ZR 0, ZR 0, ZR 0] [] 3.
+Example conv0 : STP [ZR 0, ZR 1, ZR 2] (0,$[]) 3.
 Proof. reflexivity. Qed.
+
+Example conv0' : ~STP [ZR 0, ZR 1, ZR 2] (0,$[]) 2.
+Proof. discriminate. Qed.
  
-Example conv1 : HALTS [ZR 0,ZR 0,ZR 0] [].
+Example conv1 : HALTS [ZR 0,ZR 0,ZR 0] (0,$[]).
 Proof. exists 3. reflexivity. Qed.
 
 
 
 (* Prove this can't halt by induction? *)
-Example conv2 : DIVERGES [JP 0 0 0] [].
+Example conv2 : DIVERGES [JP 0 0 0] (0,$[]).
 Proof.
- unfold DIVERGES. 
  admit.
+
+
+Lemma fixpoint : forall (t:nat) (P:program) (c:config),
+  EXEC_STEP P c = c ->
+  EXEC_STEPS t P c = c.
+Proof.
+  intros.
+  induction t. reflexivity. 
+  simpl. rewrite -> IHt. rewrite -> H. reflexivity. Qed.
+
+
+Lemma fixpoint_diverge : forall (t:nat) (P:program) (c:config),
+  EXEC_STEP P c = c -> 
+  (true = Final P c) = STP P c t.
+Proof.
+  intros.
+  unfold STP.
+  rewrite fixpoint.
+  reflexivity.
+  rewrite H. reflexivity. Qed.
+
+Example conv2' : forall (t:nat), ~(STP [JP 0 0 0] (0,$[]) t). 
+Proof.
+ intros.
+ unfold STP.
+ rewrite fixpoint.
+ discriminate.
+ reflexivity. Qed.
+
